fairneris/partial_termination.v
@@ -1,444 +1,444 @@
-From Paco Require Import pacotac.
-From stdpp Require Import finite.
-From iris.proofmode Require Import proofmode.
-From trillium Require Import adequacy.
-From fairneris Require Import fairness retransmit_model.
-From fairneris.aneris_lang Require Import aneris_lang resources.
-From fairneris.aneris_lang.state_interp Require Import state_interp_def.
-From fairneris.aneris_lang.state_interp Require Import state_interp_config_wp.
-From fairneris.aneris_lang.state_interp Require Import state_interp.
-From fairneris.aneris_lang.program_logic Require Import aneris_weakestpre.
-From fairneris Require Import from_locale_utils trace_utils ltl_lite.
+(* From Paco Require Import pacotac. *)
+(* From stdpp Require Import finite. *)
+(* From iris.proofmode Require Import proofmode. *)
+(* From trillium Require Import adequacy. *)
+(* From fairneris Require Import fairness retransmit_model. *)
+(* From fairneris.aneris_lang Require Import aneris_lang resources. *)
+(* From fairneris.aneris_lang.state_interp Require Import state_interp_def. *)
+(* From fairneris.aneris_lang.state_interp Require Import state_interp_config_wp. *)
+(* From fairneris.aneris_lang.state_interp Require Import state_interp. *)
+(* From fairneris.aneris_lang.program_logic Require Import aneris_weakestpre. *)
+(* From fairneris Require Import from_locale_utils trace_utils ltl_lite. *)
 
-Definition snd_proj {A1 A2 B1 B2} (l : (A1 * A2) + (B1 * B2)) : (A2 + B2) :=
-  sum_map snd snd l.
+(* Definition snd_proj {A1 A2 B1 B2} (l : (A1 * A2) + (B1 * B2)) : (A2 + B2) := *)
+(*   sum_map snd snd l. *)
 
-Definition ex_send_filter msg : cfg aneris_lang → option $ ex_label aneris_lang → Prop :=
-  λ _ l, option_map (sum_map snd id) l = Some $ inl $ Some msg.
-Instance ex_send_filter_decision msg st l : Decision (ex_send_filter msg st l).
-Proof. apply make_decision. Qed.
+(* Definition ex_send_filter msg : cfg aneris_lang → option $ ex_label aneris_lang → Prop := *)
+(*   λ _ l, option_map (sum_map snd id) l = Some $ inl $ Some msg. *)
+(* Instance ex_send_filter_decision msg st l : Decision (ex_send_filter msg st l). *)
+(* Proof. apply make_decision. Qed. *)
 
-Definition ex_deliver_filter msg : cfg aneris_lang → option $ ex_label aneris_lang → Prop :=
-  λ _ l, option_map (sum_map snd id) l = Some $ inr $ Some msg.
-Instance ex_deliver_filter_decision msg st l : Decision (ex_deliver_filter msg st l).
-Proof. apply make_decision. Qed.
+(* Definition ex_deliver_filter msg : cfg aneris_lang → option $ ex_label aneris_lang → Prop := *)
+(*   λ _ l, option_map (sum_map snd id) l = Some $ inr $ Some msg. *)
+(* Instance ex_deliver_filter_decision msg st l : Decision (ex_deliver_filter msg st l). *)
+(* Proof. apply make_decision. Qed. *)
 
-Definition retransmit_fair_network_delivery_ex msg : extrace aneris_lang → Prop :=
-  □ (□◊↓ex_send_filter msg → ◊↓ex_deliver_filter msg).
+(* Definition retransmit_fair_network_delivery_ex msg : extrace aneris_lang → Prop := *)
+(*   □ (□◊↓ex_send_filter msg → ◊↓ex_deliver_filter msg). *)
 
-Definition retransmit_fair_network_ex (extr : extrace aneris_lang) : Prop :=
-  ∀ msg, retransmit_fair_network_delivery_ex msg extr.
+(* Definition retransmit_fair_network_ex (extr : extrace aneris_lang) : Prop := *)
+(*   ∀ msg, retransmit_fair_network_delivery_ex msg extr. *)
 
-(* TODO: Clean up this definition (annoying to state lemmas about,
-         due to separate labels) *)
-Definition live_tid (c : cfg aneris_lang) (δ : retransmit_state)
-  (ℓ:retransmit_node_role) (ζ:locale aneris_lang) : Prop :=
-  roles_match ζ ℓ →
-  role_enabled_model (ℓ:fmrole retransmit_fair_model) δ → locale_enabled ζ c.
+(* (* TODO: Clean up this definition (annoying to state lemmas about, *)
+(*          due to separate labels) *) *)
+(* Definition live_tid (c : cfg aneris_lang) (δ : retransmit_state) *)
+(*   (ℓ:retransmit_node_role) (ζ:locale aneris_lang) : Prop := *)
+(*   roles_match ζ ℓ → *)
+(*   role_enabled_model (ℓ:fmrole retransmit_fair_model) δ → locale_enabled ζ c. *)
 
-Definition live_tids (c : cfg aneris_lang) (δ : retransmit_state) : Prop :=
-  ∀ ℓ ζ, live_tid c δ ℓ ζ.
+(* Definition live_tids (c : cfg aneris_lang) (δ : retransmit_state) : Prop := *)
+(*   ∀ ℓ ζ, live_tid c δ ℓ ζ. *)
 
-Definition live_traces_match : extrace aneris_lang → mtrace → Prop :=
-  traces_match labels_match live_tids language.locale_step retransmit_trans.
+(* Definition live_traces_match : extrace aneris_lang → mtrace → Prop := *)
+(*   traces_match labels_match live_tids language.locale_step retransmit_trans. *)
 
-Lemma traces_match_cons_inv {S1 S2 L1 L2}
-      (Rℓ: L1 -> L2 -> Prop) (Rs: S1 -> S2 -> Prop)
-      (trans1: S1 -> L1 -> S1 -> Prop)
-      (trans2: S2 -> L2 -> S2 -> Prop)
-      s1 s2 l1 l2 tr1 tr2 :
-  traces_match Rℓ Rs trans1 trans2 (s1 -[l1]-> tr1) (s2 -[l2]-> tr2) ->
-  Rs s1 s2 ∧ Rℓ l1 l2.
-Proof. intros Hm. inversion Hm; done. Qed.
+(* Lemma traces_match_cons_inv {S1 S2 L1 L2} *)
+(*       (Rℓ: L1 -> L2 -> Prop) (Rs: S1 -> S2 -> Prop) *)
+(*       (trans1: S1 -> L1 -> S1 -> Prop) *)
+(*       (trans2: S2 -> L2 -> S2 -> Prop) *)
+(*       s1 s2 l1 l2 tr1 tr2 : *)
+(*   traces_match Rℓ Rs trans1 trans2 (s1 -[l1]-> tr1) (s2 -[l2]-> tr2) -> *)
+(*   Rs s1 s2 ∧ Rℓ l1 l2. *)
+(* Proof. intros Hm. inversion Hm; done. Qed. *)
 
-Lemma traces_match_valid_preserved extr mtr :
-  live_traces_match extr mtr → mtrace_valid mtr.
-Proof.
-  rewrite /mtrace_valid trace_alwaysI. intros Hmatch tr [n Hsuffix].
-  eapply traces_match_after in Hmatch as [? [? Hmatch]]; [|done].
-  by inversion Hmatch.
-Qed.
+(* Lemma traces_match_valid_preserved extr mtr : *)
+(*   live_traces_match extr mtr → mtrace_valid mtr. *)
+(* Proof. *)
+(*   rewrite /mtrace_valid trace_alwaysI. intros Hmatch tr [n Hsuffix]. *)
+(*   eapply traces_match_after in Hmatch as [? [? Hmatch]]; [|done]. *)
+(*   by inversion Hmatch. *)
+(* Qed. *)
 
-Definition extrace_fair (extr : extrace aneris_lang) :=
-  (∀ ζ, fair_scheduling_ex ζ extr) ∧ retransmit_fair_network_ex extr.
+(* Definition extrace_fair (extr : extrace aneris_lang) := *)
+(*   (∀ ζ, fair_scheduling_ex ζ extr) ∧ retransmit_fair_network_ex extr. *)
 
-Lemma labels_match_deliver_filter_impl msg s1 s2 ℓ1 ℓ2 extr mtr :
-  labels_match ℓ1 ℓ2 →
-  (↓ ex_deliver_filter msg) (s1 -[ ℓ1 ]-> extr) →
-  (↓ deliver_filter msg) (s2 -[ ℓ2 ]-> mtr).
-Proof.
-  intros Hmatch Hmtr.
-  rewrite /trace_now /pred_at /ex_deliver_filter in Hmtr.
-  rewrite /trace_now /pred_at /deliver_filter. simpl in *.
-  destruct ℓ1; simplify_eq.
-  destruct ℓ2; [done|].
-  rewrite /labels_match /locale_retransmit_label in Hmatch.
-  by simplify_eq.
-Qed.
+(* Lemma labels_match_deliver_filter_impl msg s1 s2 ℓ1 ℓ2 extr mtr : *)
+(*   labels_match ℓ1 ℓ2 → *)
+(*   (↓ ex_deliver_filter msg) (s1 -[ ℓ1 ]-> extr) → *)
+(*   (↓ deliver_filter msg) (s2 -[ ℓ2 ]-> mtr). *)
+(* Proof. *)
+(*   intros Hmatch Hmtr. *)
+(*   rewrite /trace_now /pred_at /ex_deliver_filter in Hmtr. *)
+(*   rewrite /trace_now /pred_at /deliver_filter. simpl in *. *)
+(*   destruct ℓ1; simplify_eq. *)
+(*   destruct ℓ2; [done|]. *)
+(*   rewrite /labels_match /locale_retransmit_label in Hmatch. *)
+(*   by simplify_eq. *)
+(* Qed. *)
 
-Lemma labels_match_send_filter_impl msg s1 s2 ℓ1 ℓ2 extr mtr :
-  labels_match ℓ1 ℓ2 →
-  (↓ send_filter msg) (s2 -[ ℓ2 ]-> mtr) →
-  (↓ ex_send_filter msg) (s1 -[ ℓ1 ]-> extr).
-Proof.
-  intros Hmatch Hmtr.
-  rewrite /trace_now /pred_at /send_filter in Hmtr.
-  rewrite /trace_now /pred_at /ex_send_filter. simpl in *.
-  simplify_eq.
-  destruct ℓ2; simplify_eq.
-  assert (r.2 = Some msg) as Heq1.
-  { destruct r.
-    rewrite /label_action /locale_retransmit_label in Hmtr.
-    simpl in *. by simplify_eq. }
-  destruct ℓ1; simplify_eq; last first.
-  { rewrite /labels_match /locale_retransmit_label in Hmatch.
-    simplify_eq. }
-  assert (l.2 = r.2) as Heq2.
-  { rewrite /labels_match /locale_retransmit_label in Hmatch.
-    destruct l.
-    destruct (locale_retransmit_role l); [|done].
-    simpl in *. simplify_eq. simpl. done. }
-  simpl. rewrite Heq2 Heq1. done.
-Qed.
+(* Lemma labels_match_send_filter_impl msg s1 s2 ℓ1 ℓ2 extr mtr : *)
+(*   labels_match ℓ1 ℓ2 → *)
+(*   (↓ send_filter msg) (s2 -[ ℓ2 ]-> mtr) → *)
+(*   (↓ ex_send_filter msg) (s1 -[ ℓ1 ]-> extr). *)
+(* Proof. *)
+(*   intros Hmatch Hmtr. *)
+(*   rewrite /trace_now /pred_at /send_filter in Hmtr. *)
+(*   rewrite /trace_now /pred_at /ex_send_filter. simpl in *. *)
+(*   simplify_eq. *)
+(*   destruct ℓ2; simplify_eq. *)
+(*   assert (r.2 = Some msg) as Heq1. *)
+(*   { destruct r. *)
+(*     rewrite /label_action /locale_retransmit_label in Hmtr. *)
+(*     simpl in *. by simplify_eq. } *)
+(*   destruct ℓ1; simplify_eq; last first. *)
+(*   { rewrite /labels_match /locale_retransmit_label in Hmatch. *)
+(*     simplify_eq. } *)
+(*   assert (l.2 = r.2) as Heq2. *)
+(*   { rewrite /labels_match /locale_retransmit_label in Hmatch. *)
+(*     destruct l. *)
+(*     destruct (locale_retransmit_role l); [|done]. *)
+(*     simpl in *. simplify_eq. simpl. done. } *)
+(*   simpl. rewrite Heq2 Heq1. done. *)
+(* Qed. *)
 
-Lemma fair_network_impl extr mtr :
-  live_traces_match extr mtr →
-  retransmit_fair_network_ex extr → retransmit_fair_network mtr.
-Proof.
-  rewrite /retransmit_fair_network_ex /retransmit_fair_network.
-  intros Hmatch Hfairex_network.
-  assert (mtrace_valid mtr) as Hvalid.
-  { by eapply traces_match_valid_preserved. }
-  intros msg.
-  specialize (Hfairex_network msg).
-  rewrite /retransmit_fair_network_delivery_ex in Hfairex_network.
-  rewrite trace_alwaysI in Hfairex_network.
-  rewrite /retransmit_fair_network_delivery.
-  rewrite trace_alwaysI.
-  intros mtr' [n Hmtr'].
-  pose proof Hmtr' as Hextr'.
-  eapply traces_match_after in Hextr'; [|done].
-  destruct Hextr' as (extr'&Hextr'&Hmatch').
-  specialize (Hfairex_network extr').
-  assert (trace_suffix_of extr' extr) as Hsuffix.
-  { eexists _. done. }
-  apply Hfairex_network in Hsuffix.
-  rewrite trace_impliesI.
-  rewrite trace_impliesI in Hsuffix.
-  intros Hmtr''.
-  assert ((□ ◊ ↓ ex_send_filter msg) extr') as Hextr''.
-  { rewrite trace_alwaysI.
-    intros extr'' [m Hextr''].
-    eapply traces_match_flip in Hmatch'.
-    pose proof Hextr'' as Hmtr'''.
-    eapply traces_match_after in Hmtr'''; [|done].
-    destruct Hmtr''' as (mtr''&Hmtr'''&Hmatch'').
-    rewrite trace_alwaysI in Hmtr''.
-    specialize (Hmtr'' mtr'').
-    assert (trace_suffix_of mtr'' mtr') as Hsuffix'.
-    { eexists _. done. }
-    apply Hmtr'' in Hsuffix'.
-    rewrite trace_eventuallyI in Hsuffix'.
-    destruct Hsuffix' as [mtr''' [Hsuffix' Hmtr'''']].
-    destruct Hsuffix' as [m'' Hsuffix'].
-    apply traces_match_flip in Hmatch''.
-    eapply traces_match_after in Hmatch''; [|done].
-    destruct Hmatch'' as [extr''' [Hextr''' Hmatch''']].
-    destruct mtr'''; [done|].
-    simpl in *.
-    rewrite trace_eventuallyI. exists extr'''.
-    split; [eexists _;done|].
-    destruct extr'''; [by inversion Hmatch'''|].
-    assert (labels_match ℓ0 ℓ) as Hlabels.
-    { by eapply traces_match_cons_inv. }
-    by eapply labels_match_send_filter_impl. }
-  apply Hsuffix in Hextr''.
-  rewrite trace_eventuallyI in Hextr''.
-  destruct Hextr'' as [extr'' [[m Hsuffix''] Hextr'']].
-  rewrite trace_eventuallyI.
-  eapply traces_match_flip in Hmatch'.
-  eapply traces_match_after in Hmatch'; [|done].
-  destruct Hmatch' as [mtr'' [Hmtr''' Hmatch'']].
-  exists mtr''. split; [by eexists _|].
-  destruct extr''; [done|].
-  destruct mtr''; [by inversion Hmatch''|].
-  assert (labels_match ℓ ℓ0) as Hlabels.
-  { eapply traces_match_cons_inv. apply traces_match_flip. done. }
-  by eapply labels_match_deliver_filter_impl.
-Qed.
+(* Lemma fair_network_impl extr mtr : *)
+(*   live_traces_match extr mtr → *)
+(*   retransmit_fair_network_ex extr → retransmit_fair_network mtr. *)
+(* Proof. *)
+(*   rewrite /retransmit_fair_network_ex /retransmit_fair_network. *)
+(*   intros Hmatch Hfairex_network. *)
+(*   assert (mtrace_valid mtr) as Hvalid. *)
+(*   { by eapply traces_match_valid_preserved. } *)
+(*   intros msg. *)
+(*   specialize (Hfairex_network msg). *)
+(*   rewrite /retransmit_fair_network_delivery_ex in Hfairex_network. *)
+(*   rewrite trace_alwaysI in Hfairex_network. *)
+(*   rewrite /retransmit_fair_network_delivery. *)
+(*   rewrite trace_alwaysI. *)
+(*   intros mtr' [n Hmtr']. *)
+(*   pose proof Hmtr' as Hextr'. *)
+(*   eapply traces_match_after in Hextr'; [|done]. *)
+(*   destruct Hextr' as (extr'&Hextr'&Hmatch'). *)
+(*   specialize (Hfairex_network extr'). *)
+(*   assert (trace_suffix_of extr' extr) as Hsuffix. *)
+(*   { eexists _. done. } *)
+(*   apply Hfairex_network in Hsuffix. *)
+(*   rewrite trace_impliesI. *)
+(*   rewrite trace_impliesI in Hsuffix. *)
+(*   intros Hmtr''. *)
+(*   assert ((□ ◊ ↓ ex_send_filter msg) extr') as Hextr''. *)
+(*   { rewrite trace_alwaysI. *)
+(*     intros extr'' [m Hextr'']. *)
+(*     eapply traces_match_flip in Hmatch'. *)
+(*     pose proof Hextr'' as Hmtr'''. *)
+(*     eapply traces_match_after in Hmtr'''; [|done]. *)
+(*     destruct Hmtr''' as (mtr''&Hmtr'''&Hmatch''). *)
+(*     rewrite trace_alwaysI in Hmtr''. *)
+(*     specialize (Hmtr'' mtr''). *)
+(*     assert (trace_suffix_of mtr'' mtr') as Hsuffix'. *)
+(*     { eexists _. done. } *)
+(*     apply Hmtr'' in Hsuffix'. *)
+(*     rewrite trace_eventuallyI in Hsuffix'. *)
+(*     destruct Hsuffix' as [mtr''' [Hsuffix' Hmtr'''']]. *)
+(*     destruct Hsuffix' as [m'' Hsuffix']. *)
+(*     apply traces_match_flip in Hmatch''. *)
+(*     eapply traces_match_after in Hmatch''; [|done]. *)
+(*     destruct Hmatch'' as [extr''' [Hextr''' Hmatch''']]. *)
+(*     destruct mtr'''; [done|]. *)
+(*     simpl in *. *)
+(*     rewrite trace_eventuallyI. exists extr'''. *)
+(*     split; [eexists _;done|]. *)
+(*     destruct extr'''; [by inversion Hmatch'''|]. *)
+(*     assert (labels_match ℓ0 ℓ) as Hlabels. *)
+(*     { by eapply traces_match_cons_inv. } *)
+(*     by eapply labels_match_send_filter_impl. } *)
+(*   apply Hsuffix in Hextr''. *)
+(*   rewrite trace_eventuallyI in Hextr''. *)
+(*   destruct Hextr'' as [extr'' [[m Hsuffix''] Hextr'']]. *)
+(*   rewrite trace_eventuallyI. *)
+(*   eapply traces_match_flip in Hmatch'. *)
+(*   eapply traces_match_after in Hmatch'; [|done]. *)
+(*   destruct Hmatch' as [mtr'' [Hmtr''' Hmatch'']]. *)
+(*   exists mtr''. split; [by eexists _|]. *)
+(*   destruct extr''; [done|]. *)
+(*   destruct mtr''; [by inversion Hmatch''|]. *)
+(*   assert (labels_match ℓ ℓ0) as Hlabels. *)
+(*   { eapply traces_match_cons_inv. apply traces_match_flip. done. } *)
+(*   by eapply labels_match_deliver_filter_impl. *)
+(* Qed. *)
 
-Definition retransmit_role_locale (ρ : retransmit_node_role) : locale aneris_lang :=
-  match ρ with
-  | Arole => ("0.0.0.0",0)
-  | Brole => ("0.0.0.1",0)
-  end.
+(* Definition retransmit_role_locale (ρ : retransmit_node_role) : locale aneris_lang := *)
+(*   match ρ with *)
+(*   | Arole => ("0.0.0.0",0) *)
+(*   | Brole => ("0.0.0.1",0) *)
+(*   end. *)
 
-Lemma locale_retransmit_role_cancel ρ :
-  locale_retransmit_role (retransmit_role_locale ρ) = Some ρ.
-Proof. by destruct ρ. Qed.
+(* Lemma locale_retransmit_role_cancel ρ : *)
+(*   locale_retransmit_role (retransmit_role_locale ρ) = Some ρ. *)
+(* Proof. by destruct ρ. Qed. *)
 
-Lemma fair_scheduling_impl extr mtr :
-  live_traces_match extr mtr →
-  (∀ ζ, fair_scheduling_ex ζ extr) → retransmit_fair_scheduling mtr.
-Proof.
-  rewrite /fair_scheduling_ex /retransmit_fair_scheduling.
-  intros Hmatch Hextr ρ.
-  rewrite /retransmit_fair_scheduling_mtr.
-  rewrite /trace_always_eventually_implies_now.
-  rewrite /trace_always_eventually_implies.
-  rewrite trace_alwaysI.
-  intros mtr' [n Hmtr_after]. rewrite trace_impliesI.
-  intros Hρ.
-  eapply traces_match_after in Hmatch; [|done].
-  destruct Hmatch as [extr' [Hextr_after Hmatch]].
-  specialize (Hextr (retransmit_role_locale ρ) n).
-  rewrite /pred_at in Hextr.
-  rewrite Hextr_after in Hextr.
-  assert (match extr' with
-          | ⟨ s ⟩ | s -[ _ ]-> _ => locale_enabled (retransmit_role_locale ρ) s
-          end) as Hextr'.
-  { apply traces_match_first in Hmatch.
-    destruct extr'.
-    - eapply (Hmatch ρ).
-      + destruct ρ; done.
-      + rewrite /trace_now /pred_at in Hρ. simpl in *.
-        by destruct mtr'.
-    - eapply (Hmatch ρ).
-      + destruct ρ; done.
-      + rewrite /trace_now /pred_at in Hρ. simpl in *.
-        by destruct mtr'. }
-  apply Hextr in Hextr' as [m Hextr'].
-  rewrite after_sum' Hextr_after in Hextr'.
-  destruct (after m extr') as [extr''|] eqn:Hextr_after'; last first.
-  { rewrite Hextr_after' in Hextr'. done. }
-  rewrite Hextr_after' in Hextr'.
-  rewrite trace_eventuallyI.
-  apply traces_match_flip in Hmatch.
-  eapply traces_match_after in Hmatch; [|done].
-  destruct Hmatch as [mtr'' [Hmtr_after' Hmatch]].
-  exists mtr''. split; [by eexists _|].
-  rewrite /trace_now /pred_at=> /=.
-  destruct mtr''.
-  - destruct extr''; [|by inversion Hmatch].
-    destruct Hextr' as [Hextr'|Hextr']; [|naive_solver].
-    left. intros Hs. apply Hextr'.
-    apply traces_match_first in Hmatch.
-    eapply (Hmatch ρ).
-    + destruct ρ; done.
-    + rewrite /trace_now /pred_at in Hρ. simpl in *. done.
-  - destruct extr''; [by inversion Hmatch|].
-    destruct Hextr' as [Hextr'|Hextr'].
-    { left. intros Hs. apply Hextr'.
-      apply traces_match_first in Hmatch.
-      eapply (Hmatch ρ).
-      + destruct ρ; done.
-      + rewrite /trace_now /pred_at in Hρ. simpl in *. done. }
-    right. simpl in *. simplify_eq.
-    apply traces_match_cons_inv in Hmatch as [_ Hmatch].
-    rewrite /labels_match in Hmatch.
-    destruct ℓ0 as [[ζ act]|]; [|naive_solver].
-    simpl in *. destruct Hextr'. simplify_eq.
-    rewrite locale_retransmit_role_cancel in Hmatch.
-    simpl in *. simplify_eq. done.
-Qed.
+(* Lemma fair_scheduling_impl extr mtr : *)
+(*   live_traces_match extr mtr → *)
+(*   (∀ ζ, fair_scheduling_ex ζ extr) → retransmit_fair_scheduling mtr. *)
+(* Proof. *)
+(*   rewrite /fair_scheduling_ex /retransmit_fair_scheduling. *)
+(*   intros Hmatch Hextr ρ. *)
+(*   rewrite /retransmit_fair_scheduling_mtr. *)
+(*   rewrite /trace_always_eventually_implies_now. *)
+(*   rewrite /trace_always_eventually_implies. *)
+(*   rewrite trace_alwaysI. *)
+(*   intros mtr' [n Hmtr_after]. rewrite trace_impliesI. *)
+(*   intros Hρ. *)
+(*   eapply traces_match_after in Hmatch; [|done]. *)
+(*   destruct Hmatch as [extr' [Hextr_after Hmatch]]. *)
+(*   specialize (Hextr (retransmit_role_locale ρ) n). *)
+(*   rewrite /pred_at in Hextr. *)
+(*   rewrite Hextr_after in Hextr. *)
+(*   assert (match extr' with *)
+(*           | ⟨ s ⟩ | s -[ _ ]-> _ => locale_enabled (retransmit_role_locale ρ) s *)
+(*           end) as Hextr'. *)
+(*   { apply traces_match_first in Hmatch. *)
+(*     destruct extr'. *)
+(*     - eapply (Hmatch ρ). *)
+(*       + destruct ρ; done. *)
+(*       + rewrite /trace_now /pred_at in Hρ. simpl in *. *)
+(*         by destruct mtr'. *)
+(*     - eapply (Hmatch ρ). *)
+(*       + destruct ρ; done. *)
+(*       + rewrite /trace_now /pred_at in Hρ. simpl in *. *)
+(*         by destruct mtr'. } *)
+(*   apply Hextr in Hextr' as [m Hextr']. *)
+(*   rewrite after_sum' Hextr_after in Hextr'. *)
+(*   destruct (after m extr') as [extr''|] eqn:Hextr_after'; last first. *)
+(*   { rewrite Hextr_after' in Hextr'. done. } *)
+(*   rewrite Hextr_after' in Hextr'. *)
+(*   rewrite trace_eventuallyI. *)
+(*   apply traces_match_flip in Hmatch. *)
+(*   eapply traces_match_after in Hmatch; [|done]. *)
+(*   destruct Hmatch as [mtr'' [Hmtr_after' Hmatch]]. *)
+(*   exists mtr''. split; [by eexists _|]. *)
+(*   rewrite /trace_now /pred_at=> /=. *)
+(*   destruct mtr''. *)
+(*   - destruct extr''; [|by inversion Hmatch]. *)
+(*     destruct Hextr' as [Hextr'|Hextr']; [|naive_solver]. *)
+(*     left. intros Hs. apply Hextr'. *)
+(*     apply traces_match_first in Hmatch. *)
+(*     eapply (Hmatch ρ). *)
+(*     + destruct ρ; done. *)
+(*     + rewrite /trace_now /pred_at in Hρ. simpl in *. done. *)
+(*   - destruct extr''; [by inversion Hmatch|]. *)
+(*     destruct Hextr' as [Hextr'|Hextr']. *)
+(*     { left. intros Hs. apply Hextr'. *)
+(*       apply traces_match_first in Hmatch. *)
+(*       eapply (Hmatch ρ). *)
+(*       + destruct ρ; done. *)
+(*       + rewrite /trace_now /pred_at in Hρ. simpl in *. done. } *)
+(*     right. simpl in *. simplify_eq. *)
+(*     apply traces_match_cons_inv in Hmatch as [_ Hmatch]. *)
+(*     rewrite /labels_match in Hmatch. *)
+(*     destruct ℓ0 as [[ζ act]|]; [|naive_solver]. *)
+(*     simpl in *. destruct Hextr'. simplify_eq. *)
+(*     rewrite locale_retransmit_role_cancel in Hmatch. *)
+(*     simpl in *. simplify_eq. done. *)
+(* Qed. *)
 
-Lemma traces_match_fairness_preserved extr mtr :
-  live_traces_match extr mtr →
-  extrace_fair extr → mtrace_fair mtr.
-Proof.
-  intros Hmatch [Hfairex_sched Hfairex_network].
-  split; [by eapply fair_scheduling_impl|by eapply fair_network_impl].
-Qed.
+(* Lemma traces_match_fairness_preserved extr mtr : *)
+(*   live_traces_match extr mtr → *)
+(*   extrace_fair extr → mtrace_fair mtr. *)
+(* Proof. *)
+(*   intros Hmatch [Hfairex_sched Hfairex_network]. *)
+(*   split; [by eapply fair_scheduling_impl|by eapply fair_network_impl]. *)
+(* Qed. *)
 
-(* TODO: This needs updating to capture spawned threads *)
-(* TODO: Can likely get rid of right disjunct if we assume maximality *)
-Definition extrace_terminating_locale (ζ : locale aneris_lang) (tr : extrace aneris_lang) : Prop :=
-  (◊↓λ st _, ¬ locale_enabled ζ st) tr ∨ ¬ infinite_trace tr.
+(* (* TODO: This needs updating to capture spawned threads *) *)
+(* (* TODO: Can likely get rid of right disjunct if we assume maximality *) *)
+(* Definition extrace_terminating_locale (ζ : locale aneris_lang) (tr : extrace aneris_lang) : Prop := *)
+(*   (◊↓λ st _, ¬ locale_enabled ζ st) tr ∨ ¬ infinite_trace tr. *)
 
-Lemma disabled_always_disabled ρ (mtr : mtrace) :
-  mtrace_valid mtr →
-  (↓λ st _, ρ ∉ retransmit_live_roles st) mtr →
-  (□↓λ st _, ρ ∉ retransmit_live_roles st) mtr.
-Proof.
-  intros Hvalid Hmtr.
-  rewrite trace_alwaysI.
-  intros mtr' [m Hafter].
-  revert mtr' Hmtr Hafter Hvalid.
-  induction m as [|m Hm]; intros mtr' Hmtr Hafter Hvalid.
-  { simpl in *. simplify_eq. done. }
-  replace (S m) with (m + 1) in Hafter by lia.
-  rewrite after_sum' in Hafter.
-  destruct (after m mtr) as [mtr''|] eqn:Heqn; [|done].
-  eapply Hm in Hmtr; [|done|done].
-  eapply trace_always_suffix_of in Hvalid; [|by eexists _].
-  apply trace_always_elim in Hvalid.
-  destruct mtr''; [done|]. simpl in *. simplify_eq.
-  rewrite /trace_now /pred_at in Hmtr. simpl in *.
-  rewrite /trace_now /pred_at. simpl in *.
-  destruct mtr'.
-  - inversion Hvalid; try set_solver.
-  - inversion Hvalid; try set_solver.
-Qed.
+(* Lemma disabled_always_disabled ρ (mtr : mtrace) : *)
+(*   mtrace_valid mtr → *)
+(*   (↓λ st _, ρ ∉ retransmit_live_roles st) mtr → *)
+(*   (□↓λ st _, ρ ∉ retransmit_live_roles st) mtr. *)
+(* Proof. *)
+(*   intros Hvalid Hmtr. *)
+(*   rewrite trace_alwaysI. *)
+(*   intros mtr' [m Hafter]. *)
+(*   revert mtr' Hmtr Hafter Hvalid. *)
+(*   induction m as [|m Hm]; intros mtr' Hmtr Hafter Hvalid. *)
+(*   { simpl in *. simplify_eq. done. } *)
+(*   replace (S m) with (m + 1) in Hafter by lia. *)
+(*   rewrite after_sum' in Hafter. *)
+(*   destruct (after m mtr) as [mtr''|] eqn:Heqn; [|done]. *)
+(*   eapply Hm in Hmtr; [|done|done]. *)
+(*   eapply trace_always_suffix_of in Hvalid; [|by eexists _]. *)
+(*   apply trace_always_elim in Hvalid. *)
+(*   destruct mtr''; [done|]. simpl in *. simplify_eq. *)
+(*   rewrite /trace_now /pred_at in Hmtr. simpl in *. *)
+(*   rewrite /trace_now /pred_at. simpl in *. *)
+(*   destruct mtr'. *)
+(*   - inversion Hvalid; try set_solver. *)
+(*   - inversion Hvalid; try set_solver. *)
+(* Qed. *)
 
-Lemma retransmit_trace_valid_live ρ (mtr : mtrace) :
-  mtrace_valid mtr →
-  (↓ (λ (_ : retransmit_state) (ℓ : option retransmit_label),
-        option_map label_role ℓ = Some (inl ρ))) mtr →
-  ρ ∈ retransmit_live_roles (trfirst mtr).
-Proof.
-  intros Hvalid Hlabel.
-  apply trace_always_elim in Hvalid.
-  destruct mtr; [done|].
-  rewrite /trace_now /pred_at in Hlabel. simpl in *.
-  inversion Hvalid; set_solver.
-Qed.
+(* Lemma retransmit_trace_valid_live ρ (mtr : mtrace) : *)
+(*   mtrace_valid mtr → *)
+(*   (↓ (λ (_ : retransmit_state) (ℓ : option retransmit_label), *)
+(*         option_map label_role ℓ = Some (inl ρ))) mtr → *)
+(*   ρ ∈ retransmit_live_roles (trfirst mtr). *)
+(* Proof. *)
+(*   intros Hvalid Hlabel. *)
+(*   apply trace_always_elim in Hvalid. *)
+(*   destruct mtr; [done|]. *)
+(*   rewrite /trace_now /pred_at in Hlabel. simpl in *. *)
+(*   inversion Hvalid; set_solver. *)
+(* Qed. *)
 
-(* TODO: Prove using logic laws instead. *)
-Lemma not_infinite_terminating_trace {S L} (tr : trace S L) :
-  ¬ infinite_trace tr → terminating_trace tr.
-Proof.
-  intros Hinf. epose proof (infinite_or_finite tr) as [?|?]; done.
-Qed.
+(* (* TODO: Prove using logic laws instead. *) *)
+(* Lemma not_infinite_terminating_trace {S L} (tr : trace S L) : *)
+(*   ¬ infinite_trace tr → terminating_trace tr. *)
+(* Proof. *)
+(*   intros Hinf. epose proof (infinite_or_finite tr) as [?|?]; done. *)
+(* Qed. *)
 
-Lemma trace_always_mono_strong_alt
-      {S1 S2 L1 L2}
-      (P : trace S1 L1 → Prop)
-      (Q : trace S2 L2 → Prop)
-      Rℓ Rs trans1 trans2
-      (tr1 : trace S1 L1) (tr2 : trace S2 L2) :
-  traces_match Rℓ Rs trans1 trans2 tr1 tr2 →
-  (∀ tr1' tr2', traces_match Rℓ Rs trans1 trans2 tr1' tr2' →
-                (P tr1') → (Q tr2')) →
-  (□ P) tr1 → (□ Q) tr2.
-Proof.
-  rewrite !trace_alwaysI. intros Hmatch Himpl HP1 tr2' [n Hafter2].
-  eapply traces_match_after in Hmatch as [tr1' [Hafter1 Hmatch]]; [|done].
-  eapply Himpl; [done|]. apply HP1. by eexists _.
-Qed.
+(* Lemma trace_always_mono_strong_alt *)
+(*       {S1 S2 L1 L2} *)
+(*       (P : trace S1 L1 → Prop) *)
+(*       (Q : trace S2 L2 → Prop) *)
+(*       Rℓ Rs trans1 trans2 *)
+(*       (tr1 : trace S1 L1) (tr2 : trace S2 L2) : *)
+(*   traces_match Rℓ Rs trans1 trans2 tr1 tr2 → *)
+(*   (∀ tr1' tr2', traces_match Rℓ Rs trans1 trans2 tr1' tr2' → *)
+(*                 (P tr1') → (Q tr2')) → *)
+(*   (□ P) tr1 → (□ Q) tr2. *)
+(* Proof. *)
+(*   rewrite !trace_alwaysI. intros Hmatch Himpl HP1 tr2' [n Hafter2]. *)
+(*   eapply traces_match_after in Hmatch as [tr1' [Hafter1 Hmatch]]; [|done]. *)
+(*   eapply Himpl; [done|]. apply HP1. by eexists _. *)
+(* Qed. *)
 
-Lemma trace_eventually_mono_strong_alt
-      {S1 S2 L1 L2}
-      (P : trace S1 L1 → Prop)
-      (Q : trace S2 L2 → Prop)
-      Rℓ Rs trans1 trans2
-      (tr1 : trace S1 L1) (tr2 : trace S2 L2) :
-  traces_match Rℓ Rs trans1 trans2 tr1 tr2 →
-  (∀ tr1' tr2', traces_match Rℓ Rs trans1 trans2 tr1' tr2' →
-                (P tr1') → (Q tr2')) →
-  (◊ P) tr1 → (◊ Q) tr2.
-Proof.
-  rewrite !trace_eventuallyI. intros Hmatch Himpl [tr1' [[n Hafter1] HP1]].
-  eapply traces_match_flip in Hmatch.
-  eapply traces_match_after in Hmatch as [tr2' [Hafter2 Hmatch]]; [|done].
-  exists tr2'. split; [by eexists _|].
-  apply traces_match_flip in Hmatch. by eapply Himpl.
-Qed.
+(* Lemma trace_eventually_mono_strong_alt *)
+(*       {S1 S2 L1 L2} *)
+(*       (P : trace S1 L1 → Prop) *)
+(*       (Q : trace S2 L2 → Prop) *)
+(*       Rℓ Rs trans1 trans2 *)
+(*       (tr1 : trace S1 L1) (tr2 : trace S2 L2) : *)
+(*   traces_match Rℓ Rs trans1 trans2 tr1 tr2 → *)
+(*   (∀ tr1' tr2', traces_match Rℓ Rs trans1 trans2 tr1' tr2' → *)
+(*                 (P tr1') → (Q tr2')) → *)
+(*   (◊ P) tr1 → (◊ Q) tr2. *)
+(* Proof. *)
+(*   rewrite !trace_eventuallyI. intros Hmatch Himpl [tr1' [[n Hafter1] HP1]]. *)
+(*   eapply traces_match_flip in Hmatch. *)
+(*   eapply traces_match_after in Hmatch as [tr2' [Hafter2 Hmatch]]; [|done]. *)
+(*   exists tr2'. split; [by eexists _|]. *)
+(*   apply traces_match_flip in Hmatch. by eapply Himpl. *)
+(* Qed. *)
 
-Lemma terminating_role_preserved ρ ζ mtr extr :
-  extrace_fair extr →
-  live_traces_match extr mtr →
-  roles_match ζ ρ →
-  retransmit_terminating_role ρ mtr →
-  extrace_terminating_locale ζ extr.
-Proof.
-  intros Hfair Hmatch Hroles Hmtr.
-  assert (extrace_terminating_locale ζ extr ∨
-           ¬ extrace_terminating_locale ζ extr) as HEM.
-  { by apply ExcludedMiddle. }
-  destruct HEM as [|Hextr]; [done|]. exfalso.
-  apply Classical_Prop.not_or_and in Hextr as [Hextr Hinf].
-  assert ((□ ↓ (λ st _, locale_enabled ζ st)) extr) as Hextr'.
-  { apply trace_always_not_not_eventually in Hextr.
-    revert Hextr. apply trace_always_mono.
-    intros tr. apply trace_impliesI. intros Hextr.
-    apply trace_now_not in Hextr.
-    revert Hextr. apply trace_now_mono.
-    intros s _. intros Hextr. by apply NNP_P. }
-  assert ((□ ◊ ↓ (λ _ otid, option_map (sum_map fst id) otid = Some (inl ζ)))
-            extr) as Hex_sched.
-  { pose proof Hextr' as Hextr''.
-    revert Hextr'. apply trace_always_mono_strong.
-    intros extr' Hsuffix. rewrite trace_impliesI.
-    intros Hextr'.
-    destruct Hfair as [Hfair_sched _].
-    specialize (Hfair_sched ζ).
-    (* TODO: Bump fairness to LTL *)
-    destruct Hsuffix as [n Hafter].
-    eapply trace_implies_after in Hfair_sched; [|done].
-    apply Hfair_sched in Hextr' as [m Hextr'].
-    simpl in *.
-    apply trace_eventuallyI.
-    rewrite /pred_at in Hextr'.
-    destruct (after m extr') as [extr''|] eqn:Heqn; last first.
-    { by rewrite Heqn in Hextr'. }
-    rewrite Heqn in Hextr'.
-    exists extr''.
-    split; [by eexists _|].
-    destruct extr''.
-    - destruct Hextr'; [|naive_solver].
-      eapply trace_always_suffix_of in Hextr''; [|by eexists _].
-      eapply trace_always_suffix_of in Hextr''; [|by eexists _].
-      apply trace_always_elim in Hextr''. done.
-    - destruct Hextr'; [|naive_solver].
-      eapply trace_always_suffix_of in Hextr''; [|by eexists _].
-      eapply trace_always_suffix_of in Hextr''; [|by eexists _].
-      apply trace_always_elim in Hextr''. done.
-  }
-  assert ((□ ◊ ↓ (λ _ ℓ, option_map label_role ℓ = Some (inl ρ)))
-            mtr) as Hmtr_sched.
-  { revert Hex_sched.
-    eapply trace_always_mono_strong_alt; [done|].
-    intros extr' mtr' Hmatch'.
-    eapply trace_eventually_mono_strong_alt; [done|].
-    intros extr'' mtr'' Hmatch''.
-    rewrite /trace_now /pred_at=> /=.
-    destruct extr''; [done|].
-    destruct mtr''; [by inversion Hmatch''|].
-    apply traces_match_cons_inv in Hmatch'' as [_ Hmatch''].
-    intros Heq.
-    destruct ℓ as [[]|]; [|done].
-    rewrite /labels_match /locale_retransmit_label in Hmatch''.
-    rewrite /roles_match in Hroles.
-    simpl in *. simplify_eq.
-    destruct (locale_retransmit_role ζ) eqn:Heqn; [|done].
-    simpl in *. by simplify_eq. }
-  destruct Hmtr as [Hmtr|Hmtr]; last first.
-  { apply NNP_P in Hinf. apply not_infinite_terminating_trace in Hmtr.
-    destruct Hmtr as [n Hafter].
-    specialize (Hinf n) as [extr' Hafter'].
-    apply traces_match_flip in Hmatch.
-    eapply traces_match_after in Hmatch as [mtr'' [Hafter'' _]]; [|done].
-    by simplify_eq. }
-  clear Hinf Hextr Hextr' Hex_sched.
-  eapply trace_eventually_mono_strong in Hmtr; last first.
-  { intros mtr' Hsuffix Hmtr'.
-    eapply disabled_always_disabled; [|done].
-    eapply trace_always_suffix_of; [done|].
-    by eapply traces_match_valid_preserved. }
-  rewrite trace_eventuallyI in Hmtr.
-  destruct Hmtr as [mtr' [Hmtr_suffix Hmtr']].
-  rewrite trace_alwaysI in Hmtr_sched.
-  specialize (Hmtr_sched mtr' Hmtr_suffix).
-  rewrite trace_eventuallyI in Hmtr_sched.
-  destruct Hmtr_sched as [mtr'' [Hmtr_suffix' Hmtr'']].
-  rewrite trace_alwaysI in Hmtr'.
-  specialize (Hmtr' mtr'' Hmtr_suffix').
-  assert (mtrace_valid mtr'').
-  { eapply trace_always_suffix_of; [done|].
-    eapply trace_always_suffix_of; [done|].
-    by eapply traces_match_valid_preserved. }
-  apply retransmit_trace_valid_live in Hmtr''; [|done].
-  by destruct mtr''.
-Qed.
+(* Lemma terminating_role_preserved ρ ζ mtr extr : *)
+(*   extrace_fair extr → *)
+(*   live_traces_match extr mtr → *)
+(*   roles_match ζ ρ → *)
+(*   retransmit_terminating_role ρ mtr → *)
+(*   extrace_terminating_locale ζ extr. *)
+(* Proof. *)
+(*   intros Hfair Hmatch Hroles Hmtr. *)
+(*   assert (extrace_terminating_locale ζ extr ∨ *)
+(*            ¬ extrace_terminating_locale ζ extr) as HEM. *)
+(*   { by apply ExcludedMiddle. } *)
+(*   destruct HEM as [|Hextr]; [done|]. exfalso. *)
+(*   apply Classical_Prop.not_or_and in Hextr as [Hextr Hinf]. *)
+(*   assert ((□ ↓ (λ st _, locale_enabled ζ st)) extr) as Hextr'. *)
+(*   { apply trace_always_not_not_eventually in Hextr. *)
+(*     revert Hextr. apply trace_always_mono. *)
+(*     intros tr. apply trace_impliesI. intros Hextr. *)
+(*     apply trace_now_not in Hextr. *)
+(*     revert Hextr. apply trace_now_mono. *)
+(*     intros s _. intros Hextr. by apply NNP_P. } *)
+(*   assert ((□ ◊ ↓ (λ _ otid, option_map (sum_map fst id) otid = Some (inl ζ))) *)
+(*             extr) as Hex_sched. *)
+(*   { pose proof Hextr' as Hextr''. *)
+(*     revert Hextr'. apply trace_always_mono_strong. *)
+(*     intros extr' Hsuffix. rewrite trace_impliesI. *)
+(*     intros Hextr'. *)
+(*     destruct Hfair as [Hfair_sched _]. *)
+(*     specialize (Hfair_sched ζ). *)
+(*     (* TODO: Bump fairness to LTL *) *)
+(*     destruct Hsuffix as [n Hafter]. *)
+(*     eapply trace_implies_after in Hfair_sched; [|done]. *)
+(*     apply Hfair_sched in Hextr' as [m Hextr']. *)
+(*     simpl in *. *)
+(*     apply trace_eventuallyI. *)
+(*     rewrite /pred_at in Hextr'. *)
+(*     destruct (after m extr') as [extr''|] eqn:Heqn; last first. *)
+(*     { by rewrite Heqn in Hextr'. } *)
+(*     rewrite Heqn in Hextr'. *)
+(*     exists extr''. *)
+(*     split; [by eexists _|]. *)
+(*     destruct extr''. *)
+(*     - destruct Hextr'; [|naive_solver]. *)
+(*       eapply trace_always_suffix_of in Hextr''; [|by eexists _]. *)
+(*       eapply trace_always_suffix_of in Hextr''; [|by eexists _]. *)
+(*       apply trace_always_elim in Hextr''. done. *)
+(*     - destruct Hextr'; [|naive_solver]. *)
+(*       eapply trace_always_suffix_of in Hextr''; [|by eexists _]. *)
+(*       eapply trace_always_suffix_of in Hextr''; [|by eexists _]. *)
+(*       apply trace_always_elim in Hextr''. done. *)
+(*   } *)
+(*   assert ((□ ◊ ↓ (λ _ ℓ, option_map label_role ℓ = Some (inl ρ))) *)
+(*             mtr) as Hmtr_sched. *)
+(*   { revert Hex_sched. *)
+(*     eapply trace_always_mono_strong_alt; [done|]. *)
+(*     intros extr' mtr' Hmatch'. *)
+(*     eapply trace_eventually_mono_strong_alt; [done|]. *)
+(*     intros extr'' mtr'' Hmatch''. *)
+(*     rewrite /trace_now /pred_at=> /=. *)
+(*     destruct extr''; [done|]. *)
+(*     destruct mtr''; [by inversion Hmatch''|]. *)
+(*     apply traces_match_cons_inv in Hmatch'' as [_ Hmatch'']. *)
+(*     intros Heq. *)
+(*     destruct ℓ as [[]|]; [|done]. *)
+(*     rewrite /labels_match /locale_retransmit_label in Hmatch''. *)
+(*     rewrite /roles_match in Hroles. *)
+(*     simpl in *. simplify_eq. *)
+(*     destruct (locale_retransmit_role ζ) eqn:Heqn; [|done]. *)
+(*     simpl in *. by simplify_eq. } *)
+(*   destruct Hmtr as [Hmtr|Hmtr]; last first. *)
+(*   { apply NNP_P in Hinf. apply not_infinite_terminating_trace in Hmtr. *)
+(*     destruct Hmtr as [n Hafter]. *)
+(*     specialize (Hinf n) as [extr' Hafter']. *)
+(*     apply traces_match_flip in Hmatch. *)
+(*     eapply traces_match_after in Hmatch as [mtr'' [Hafter'' _]]; [|done]. *)
+(*     by simplify_eq. } *)
+(*   clear Hinf Hextr Hextr' Hex_sched. *)
+(*   eapply trace_eventually_mono_strong in Hmtr; last first. *)
+(*   { intros mtr' Hsuffix Hmtr'. *)
+(*     eapply disabled_always_disabled; [|done]. *)
+(*     eapply trace_always_suffix_of; [done|]. *)
+(*     by eapply traces_match_valid_preserved. } *)
+(*   rewrite trace_eventuallyI in Hmtr. *)
+(*   destruct Hmtr as [mtr' [Hmtr_suffix Hmtr']]. *)
+(*   rewrite trace_alwaysI in Hmtr_sched. *)
+(*   specialize (Hmtr_sched mtr' Hmtr_suffix). *)
+(*   rewrite trace_eventuallyI in Hmtr_sched. *)
+(*   destruct Hmtr_sched as [mtr'' [Hmtr_suffix' Hmtr'']]. *)
+(*   rewrite trace_alwaysI in Hmtr'. *)
+(*   specialize (Hmtr' mtr'' Hmtr_suffix'). *)
+(*   assert (mtrace_valid mtr''). *)
+(*   { eapply trace_always_suffix_of; [done|]. *)
+(*     eapply trace_always_suffix_of; [done|]. *)
+(*     by eapply traces_match_valid_preserved. } *)
+(*   apply retransmit_trace_valid_live in Hmtr''; [|done]. *)
+(*   by destruct mtr''. *)
+(* Qed. *)
 
-Lemma fair_extrace_terminate extr mtr :
-  live_traces_match extr mtr →
-  extrace_valid extr → extrace_fair extr →
-  extrace_terminating_locale localeB extr.
-Proof.
-  intros Hmatch Hvalid Hfair.
-  eapply terminating_role_preserved; [done|done|done|].
-  apply retransmit_fair_traces_terminate;
-    [by eapply traces_match_valid_preserved|].
-  by eapply traces_match_fairness_preserved.
-Qed.
+(* Lemma fair_extrace_terminate extr mtr : *)
+(*   live_traces_match extr mtr → *)
+(*   extrace_valid extr → extrace_fair extr → *)
+(*   extrace_terminating_locale localeB extr. *)
+(* Proof. *)
+(*   intros Hmatch Hvalid Hfair. *)
+(*   eapply terminating_role_preserved; [done|done|done|]. *)
+(*   apply retransmit_fair_traces_terminate; *)
+(*     [by eapply traces_match_valid_preserved|]. *)
+(*   by eapply traces_match_fairness_preserved. *)
+(* Qed. *)
